WIP

code/ecdsap256/Hacl.Impl.P256.Primitives.fst
@@ -22,6 +22,46 @@ open Hacl.Impl.P256.Signature.Common
 #set-options "--fuel 0 --ifuel 0 --z3rlimit 200"
 
 
+val _toForm: i:lbuffer uint8 (size 32) -> o:felem -> Stack unit
+  (requires fun h -> live h i /\ live h o /\ disjoint i o)
+  (ensures  fun h0 _ h1 ->
+    modifies (loc o) h0 h1 /\ as_nat h1 o == nat_from_bytes_be (as_seq h0 i))
+
+let _toForm i o = 
+    let h0 = ST.get() in 
+  toUint64ChangeEndian i o;
+    let h1 = ST.get() in 
+  changeEndianLemma (uints_from_bytes_be (as_seq h0 i));
+  uints_from_bytes_be_nat_lemma #U64 #_ #4 (as_seq h0 i);
+  lemma_core_0 o h1
+
+
+val toFormPoint: i: lbuffer uint8 (size 64) -> result: point -> Stack unit 
+  (requires fun h -> live h i /\ live h result /\ disjoint i result)
+  (ensures fun h0 _ h1 -> modifies (loc result) h0 h1 /\
+    (
+      let pointScalarXSeq = nat_from_bytes_be (as_seq h1 (gsub i (size 0) (size 32))) in 
+      let pointScalarYSeq = nat_from_bytes_be (as_seq h1 (gsub i (size 32) (size 32))) in 
+     
+      let x, y, z = point_x_as_nat h1 result, point_y_as_nat h1 result, point_z_as_nat h1 result in 
+      let pointJacX, pointJacY, pointJacZ = toJacobianCoordinates (pointScalarXSeq, pointScalarYSeq) in 
+      x == pointJacX /\ y == pointJacY /\ z == pointJacZ))
+
+      
+let toFormPoint i p = 
+  let pointScalarX = sub i (size 0) (size 32) in 
+  let pointScalarY = sub i (size 32) (size 32) in 
+
+  let pointX = sub p (size 0) (size 4) in 
+  let pointY = sub p (size 4) (size 4) in 
+  let pointZ = sub p (size 8) (size 4) in 
+
+  _toForm pointScalarX pointX;
+  _toForm pointScalarY pointY;
+  uploadOneImpl pointZ
+
+
+
 inline_for_extraction noextract
 val secretToPublic:
     result:lbuffer uint8 (size 64)
@@ -36,6 +76,7 @@ val secretToPublic:
     r == flag /\
     as_seq h1 (gsub result (size 0) (size 32)) == pointX /\
     as_seq h1 (gsub result (size 32) (size 32)) == pointY)
+    
 
 let secretToPublic result scalar = 
     push_frame();
@@ -50,6 +91,7 @@ let secretToPublic result scalar =
   let flag = isPointAtInfinityPrivate resultBuffer in
 
   let h0 = ST.get() in
+
   changeEndian resultBufferX;
   changeEndian resultBufferY;
 
@@ -73,7 +115,8 @@ let secretToPublic result scalar =
 (*
   This function provides a raw implementation of the secrettopublic function. 
   It doesnot provide the verification that the point gotten at the result doesnot belong to infinity.
-  We strongly encourage you to use this function only if you understand what you´re doing.
+  We strongly discourage you to use this function unless you understand what you´re doing.
+  A. 
 *)
 
 inline_for_extraction noextract
@@ -120,43 +163,41 @@ let secretToPublicRaw result scalar =
 
 
 val _scalarMult:
-    result:lbuffer uint64 (size 12) 
-  -> pubKey:lbuffer uint64 (size 8) 
+    result: point 
+  -> pubKey: point
   -> scalar: lbuffer uint8 (size 32) 
   -> Stack uint64
-    (requires fun h -> 
-      live h result /\ live h pubKey /\ live h scalar /\
-      disjoint result pubKey /\ disjoint result scalar /\
-      as_nat h (gsub result (size 0) (size 4)) == 0 /\
-      as_nat h (gsub result (size 4) (size 4)) == 0)
-    (ensures fun h0 r h1 -> 
-      modifies (loc result) h0 h1 /\
-      (let x, y = as_nat h0 (gsub pubKey (size 0) (size 4)), as_nat h0 (gsub pubKey (size 4) (size 4)) in
-       let x3, y3, z3 = point_x_as_nat h1 result, point_y_as_nat h1 result, point_z_as_nat h1 result in
-       let pointJacX, pointJacY, pointJacZ = toJacobianCoordinates (x, y) in
-       if not (verifyQValidCurvePointSpec (pointJacX, pointJacY, pointJacZ)) then
-         uint_v r = maxint U64 /\ x3 == 0 /\ y3 == 0
-       else
-        x3 < prime256 /\ y3 < prime256 /\ z3 < prime256 /\
-        (let xN, yN, zN = scalar_multiplication (as_seq h0 scalar) (pointJacX, pointJacY, pointJacZ) in
-         xN == x3 /\ yN == y3 /\ zN == z3 /\
-         (if isPointAtInfinity (xN, yN, zN) then
-           uint_v r = maxint U64
-         else
-           uint_v r = 0))))
+  (requires fun h -> 
+      live h result /\ live h pubKey /\ live h scalar /\ 
+      disjoint result pubKey /\ disjoint result scalar /\ disjoint pubKey scalar /\ (
+      as_nat h (gsub pubKey (size 0) (size 4)) < prime256 /\
+      as_nat h (gsub pubKey (size 4) (size 4)) < prime256 /\
+      as_nat h (gsub pubKey (size 8) (size 4)) == 1))
+  (ensures fun h0 r h1 ->  modifies (loc result |+| loc pubKey) h0 h1  /\ (
+    let x, y, z = as_nat h0 (gsub pubKey (size 0) (size 4)), as_nat h0 (gsub pubKey (size 4) (size 4)), as_nat h0 (gsub pubKey (size 8) (size 4)) in
+    let x3, y3, z3 = point_x_as_nat h1 result, point_y_as_nat h1 result, point_z_as_nat h1 result in
+    if not (verifyQValidCurvePointSpec (x, y, z)) then
+      uint_v r = maxint U64 /\ x3 == point_x_as_nat h0 result /\ y3 == point_y_as_nat h0 result /\ z3 == point_z_as_nat h0 result
+    else
+      x3 < prime256 /\ y3 < prime256 /\ z3 < prime256 /\ (
+      let xN, yN, zN = scalar_multiplication (as_seq h0 scalar) (x, y, z) in
+      xN == x3 /\ yN == y3 /\ zN == z3 /\ (
+      if isPointAtInfinity (xN, yN, zN) then
+	uint_v r = maxint U64
+      else
+	uint_v r = 0)))) 
 
 
 let _scalarMult result pubKey scalar =
   push_frame();
+    let h0 =  ST.get() in 
   let tempBuffer = create (size 100) (u64 0) in
-  let publicKeyBuffer = create (size 12) (u64 0) in
-  bufferToJac pubKey publicKeyBuffer;
-  let publicKeyCorrect = verifyQValidCurvePoint publicKeyBuffer tempBuffer in
+  let publicKeyCorrect = verifyQValidCurvePoint pubKey tempBuffer in
   if publicKeyCorrect then
     begin
-    scalarMultiplication publicKeyBuffer result scalar tempBuffer;
-    let flag = isPointAtInfinityPrivate result in
-    pop_frame();
+    scalarMultiplication pubKey result scalar tempBuffer;
+    let flag = isPointAtInfinityPrivate result in 
+    pop_frame(); 
     flag
     end
   else
@@ -168,33 +209,28 @@ let _scalarMult result pubKey scalar =
 
 
 val _scalarMultRaw:
-    result:lbuffer uint64 (size 12) 
-  -> pubKey:lbuffer uint64 (size 8) 
+    result:point 
+  -> pubKey: point 
   -> scalar: lbuffer uint8 (size 32) 
   -> Stack unit (requires fun h -> 
-    live h result /\ live h pubKey /\ live h scalar /\
-    disjoint result pubKey /\ disjoint result scalar /\
-    as_nat h (gsub result (size 0) (size 4)) == 0 /\
-    as_nat h (gsub result (size 4) (size 4)) == 0 /\ (
-    let x, y = as_nat h (gsub pubKey (size 0) (size 4)), as_nat h (gsub pubKey (size 4) (size 4)) in 
-    x < prime256 /\ y < prime256))
-    (ensures fun h0 _ h1 -> modifies (loc result) h0 h1 /\ (
-    let x, y = as_nat h0 (gsub pubKey (size 0) (size 4)), as_nat h0 (gsub pubKey (size 4) (size 4)) in
+    live h result /\ live h pubKey /\ live h scalar /\ 
+    disjoint result pubKey /\ disjoint result scalar /\ disjoint pubKey scalar /\ (
+    as_nat h (gsub pubKey (size 0) (size 4)) < prime256 /\
+    as_nat h (gsub pubKey (size 4) (size 4)) < prime256 /\
+    as_nat h (gsub pubKey (size 8) (size 4)) < prime256 ))
+  (ensures fun h0 r h1 ->  modifies (loc result |+| loc pubKey) h0 h1  /\ (
+    let x, y, z = as_nat h0 (gsub pubKey (size 0) (size 4)), as_nat h0 (gsub pubKey (size 4) (size 4)), as_nat h0 (gsub pubKey (size 8) (size 4)) in
     let x3, y3, z3 = point_x_as_nat h1 result, point_y_as_nat h1 result, point_z_as_nat h1 result in
-    let pointJacX, pointJacY, pointJacZ = toJacobianCoordinates (x, y) in
-    x3 < prime256 /\ y3 < prime256 /\ z3 < prime256 /\
-    (let xN, yN, zN = scalar_multiplication (as_seq h0 scalar) (pointJacX, pointJacY, pointJacZ) in
-    xN == x3 /\ yN == y3 /\ zN == z3)))
+      x3 < prime256 /\ y3 < prime256 /\ z3 < prime256 /\ (
+      let xN, yN, zN = scalar_multiplication (as_seq h0 scalar) (x, y, z) in
+      xN == x3 /\ yN == y3 /\ zN == z3)))
 
 
 let _scalarMultRaw result pubKey scalar =
   push_frame();
   let tempBuffer = create (size 100) (u64 0) in
-  let publicKeyBuffer = create (size 12) (u64 0) in
-  bufferToJac pubKey publicKeyBuffer;
-  scalarMultiplication publicKeyBuffer result scalar tempBuffer;
-  pop_frame();
-  admit()
+  scalarMultiplication pubKey result scalar tempBuffer;
+  pop_frame()
 
 
 inline_for_extraction noextract
@@ -226,24 +262,8 @@ let scalarMult result pubKey scalar =
   let resultX = sub result (size 0) (size 32) in
   let resultY = sub result (size 32) (size 32) in
 
-  let publicKeyAsFelem = create (size 8) (u64 0) in
-  let publicKeyFelemX = sub publicKeyAsFelem (size 0) (size 4) in
-  let publicKeyFelemY = sub publicKeyAsFelem (size 4) (size 4) in
-  let pubKeyX = sub pubKey (size 0) (size 32) in
-  let pubKeyY = sub pubKey (size 32) (size 32) in
-
-  toUint64ChangeEndian pubKeyX publicKeyFelemX;
-  toUint64ChangeEndian pubKeyY publicKeyFelemY;
-
-  let h1 = ST.get() in
-  lemma_core_0 publicKeyFelemX h1;
-  changeEndianLemma (uints_from_bytes_be (as_seq h0 pubKeyX));
-  uints_from_bytes_be_nat_lemma #U64 #_ #4 (as_seq h1 pubKeyX);
-
-  lemma_core_0 publicKeyFelemY h1;
-  changeEndianLemma (uints_from_bytes_be (as_seq h0 pubKeyY));
-  uints_from_bytes_be_nat_lemma #U64 #_ #4 (as_seq h1 pubKeyY);
-
+  let publicKeyAsFelem = create (size 12) (u64 0) in
+  toFormPoint pubKey publicKeyAsFelem; 
   let flag = _scalarMult resultBufferFelem publicKeyAsFelem scalar in
 
   let h2 = ST.get() in
@@ -339,32 +359,7 @@ let scalarMultRaw result pubKey scalar =
   admit()
 
 
-val _toForm: i:lbuffer uint8 (size 32) -> o:felem -> Stack unit
-  (requires fun h -> live h i /\ live h o /\ disjoint i o)
-  (ensures  fun h0 _ h1 ->
-    modifies (loc o) h0 h1 /\
-    as_seq h1 o == Spec.ECDSA.changeEndian (Lib.ByteSequence.uints_from_bytes_be (as_seq h0 i))
-  )
 
-let _toForm i o = toUint64ChangeEndian i o
-
-
-val toFormPoint: i: lbuffer uint8 (size 64) -> p: point -> Stack unit 
-  (requires fun h -> True)
-  (ensures fun h0 _ h1 -> True)
-
-
-let toFormPoint i p = 
-  let pointScalarX = sub i (size 0) (size 32) in 
-  let pointScalarY = sub i (size 32) (size 32) in 
-
-  let pointX = sub p (size 0) (size 4) in 
-  let pointY = sub p (size 4) (size 4) in 
-  let pointZ = sub p (size 8) (size 4) in 
-
-  _toForm pointScalarX pointX;
-  _toForm pointScalarY pointY;
-  uploadOneImpl pointZ
 
 
 val _fromForm: i: felem -> o: lbuffer uint8 (size 32) -> Stack unit 
